Work towards RLP decoding
Progress on #68

util/recursiveLengthPrefixScript.sml
@@ -1,5 +1,6 @@
-open HolKernel boolLib bossLib Parse
-     wordsLib wordsTheory listTheory
+open HolKernel boolLib bossLib Parse dep_rewrite
+     wordsLib wordsTheory listTheory rich_listTheory combinTheory
+     numposrepTheory arithmeticTheory logrootTheory
      vfmTypesTheory cv_transLib cv_stdTheory
 
 val _ = new_theory "recursiveLengthPrefix";
@@ -17,6 +18,27 @@ Definition num_to_be_bytes_def:
   num_to_be_bytes n : word8 list =
   if n = 0 then [] else REVERSE $ MAP n2w $ n2l 256 n
 End
+
+Definition num_of_be_bytes_def:
+  num_of_be_bytes bs =
+  l2n 256 $ MAP w2n $ REVERSE bs
+End
+
+Theorem num_of_to_be_bytes[simp]:
+  num_of_be_bytes (num_to_be_bytes n) = n
+Proof
+  rw[num_of_be_bytes_def, num_to_be_bytes_def, MAP_MAP_o, o_DEF]
+  \\ qmatch_goalsub_abbrev_tac`MAP f ls`
+  \\ `MAP f ls = MAP I ls`
+  by (
+    rw[MAP_EQ_f, Abbr`ls`, Abbr`f`]
+    \\ qspec_then`256` mp_tac n2l_BOUND
+    \\ rw[EVERY_MEM]
+    \\ first_x_assum drule \\ rw[] )
+  \\ fs[Abbr`ls`]
+  \\ irule l2n_n2l
+  \\ rw[]
+QED
 
 Definition rlp_number_def:
   rlp_number n = RLPB $ num_to_be_bytes n
@@ -63,5 +85,70 @@ Definition rlp_encode_def:
 End
 
 val () = cv_auto_trans rlp_encode_def;
+
+Definition rlp_decode_length_def:
+  rlp_decode_length bs =
+  let length = LENGTH bs in
+  if length = 0 then NONE else
+  let prefix = w2n (EL 0 bs) in
+  if prefix ≤ 0x7f
+  then SOME (0, 1, T) else
+  let strLen = prefix - 0x80 in
+  if prefix ≤ 0xb7 ∧ length > strLen
+  then SOME (1, strLen, T) else
+  let lenOfStrLen = prefix - 0xb7 in
+  let strLen = num_of_be_bytes (TAKE lenOfStrLen (TL bs)) in
+  if prefix ≤ 0xbf ∧ length > lenOfStrLen + strLen
+  then SOME (1 + lenOfStrLen, strLen, T) else
+  let listLen = prefix - 0xc0 in
+  if prefix ≤ 0xf7 ∧ length > listLen
+  then SOME (1, listLen, F) else
+  let lenOfListLen = prefix - 0xf7 in
+  let listLen = num_of_be_bytes (TAKE lenOfListLen (TL bs)) in
+  if prefix ≤ 0xff ∧ length > lenOfListLen + listLen
+  then SOME (1 + lenOfListLen, listLen, F)
+  else NONE
+End
+
+Theorem rlp_decode_length_RLPB:
+  LENGTH bs < 2 ** 64 ⇒
+  ∃offset.
+    rlp_decode_length (rlp_encode (RLPB bs)) =
+    SOME (offset, LENGTH bs, T) ∧
+    TAKE (LENGTH bs) (DROP offset (rlp_encode (RLPB bs))) = bs
+Proof
+  rw[rlp_encode_def]
+  \\ rewrite_tac[rlp_bytes_def, rlp_decode_length_def]
+  \\ IF_CASES_TAC >- rw[]
+  \\ IF_CASES_TAC >- rw[]
+  \\ qexists_tac`1 + 1 + LOG 256 (LENGTH bs)`
+  \\ reverse conj_tac
+  >- rw[DROP_APPEND, LENGTH_n2l, ADD1, TAKE_APPEND]
+  \\ BasicProvers.LET_ELIM_TAC
+  \\ IF_CASES_TAC >- gvs[Abbr`length`]
+  \\ gvs[]
+  \\ `LENGTH lengthBytes = 1 + LOG 256 (LENGTH bs)`
+  by ( rw[Abbr`lengthBytes`, LENGTH_n2l] \\ gvs[] )
+  \\ gvs[]
+  \\ `LOG 256 (LENGTH bs) ≤ 8`
+  by ( irule EXP_TO_LOG \\ gs[] )
+  \\ `prefix = LOG 256 (LENGTH bs) + 184`
+  by simp[Abbr`prefix`]
+  \\ gvs[Abbr`prefix`]
+  \\ `lengthBytes = num_to_be_bytes $ LENGTH bs`
+  by (
+    simp[Abbr`lengthBytes`, num_to_be_bytes_def]
+    \\ IF_CASES_TAC \\ gvs[MAP_REVERSE] )
+  \\ IF_CASES_TAC
+  >- gvs[Abbr`strLen'`, TAKE_APPEND]
+  \\ pop_assum mp_tac
+  \\ qpat_x_assum`_ = LENGTH _`(assume_tac o SYM)
+  \\ gvs[TAKE_APPEND, Abbr`strLen'`]
+  \\ gvs[Abbr`length`]
+  \\ Cases_on`LOG 256 (LENGTH bs) ≤ 7` >- gs[]
+  \\ `LOG 256 (LENGTH bs) = 8` by gs[] \\ gvs[]
+  \\ qspecl_then[`256`,`LENGTH bs`,`2 ** 64 - 1`]mp_tac LOG_LE_MONO
+  \\ simp[Abbr`lenOfListLen`]
+QED
 
 val _ = export_theory();
